Experiments/SR/Main.lean
@@ -3,6 +3,8 @@ import Experiments.SR.Parsing.SRParser
 
 open Trestle Parsing SRParser
 
+def ASCII_D : UInt8 := 100
+
 def printUsage : IO Unit := do
   IO.println "Usage: ./SRCheckerExe <cnf> <pf> [c]"
   IO.println ""
@@ -24,57 +26,64 @@ partial def main : List String → IO Unit
       IO.println "c CNF file too large"
       return
     else
-      let (F, nVars) ← IO.ofExcept <|
-        SRParser.parseFormula ⟨cnfContents, Nat.not_le.mp hc⟩ (RangeArray.empty : RangeArray ILit)
 
-      let bytes ← IO.FS.withFile lsrFile .read (·.readBinToEnd)
-      if h_lsr : bytes.size ≥ USize.size then
-        IO.println "c LSR file too large"
-        return
-      else
+    let (F, nVars) ← IO.ofExcept <|
+      SRParser.parseFormula ⟨cnfContents, Nat.not_le.mp hc⟩ (RangeArray.empty : RangeArray ILit)
 
-      let bytes : ByteArray' := ⟨bytes, Nat.not_le.mp h_lsr⟩
-      let size := bytes.val.size.toUSize
-      let τ := PPA.new (nVars * 2)
-      let σ := PS.new (nVars * 2)
-      let iter : USize := 0
+    -- IO.println s!"CNF Formula:"
+    -- let mut i := 0
+    -- for C in F do
+    --   i := i + 1
+    --   match C with
+    --   | none => IO.println s!"  {i}: [del]"
+    --   | some C => IO.println s!"  {i}: {Clause.toLString C}"
 
-      let rec loop (iter : USize) : SR.SRState → Except Bool (SR.SRState × USize)
-      | ⟨F, τ, σ⟩ => do
-        if iter < size then
-          -- Parse a new line
-          let ⟨lineId, iter⟩ := ByteArray.readNat bytes iter
-          let iter := ByteArray.ws bytes iter
-          let ch := ByteArray.peekc bytes iter
-          -- 'd' = 100 in ASCII
-          if ch = 100 then
-            let iter := ByteArray.skip bytes iter
-            match parseDeletionLine bytes iter with
+    let bytes ← IO.FS.withFile lsrFile .read (·.readBinToEnd)
+    if h_lsr : bytes.size ≥ USize.size then
+      IO.println "c LSR file too large"
+      return
+    else
+    let bytes : ByteArray' := ⟨bytes, Nat.not_le.mp h_lsr⟩
+    let size := bytes.val.size.toUSize
+    let τ := PPA.new (nVars * 2)
+    let σ := PS.new (nVars * 2)
+    let iter : USize := 0
+
+    let rec loop (iter : USize) : SR.SRState → Except Bool (SR.SRState × USize)
+    | ⟨F, τ, σ⟩ => do
+      if iter < size then
+        -- Parse a new line
+        let ⟨lineId, iter⟩ := ByteArray.readNat bytes iter
+        let iter := ByteArray.ws bytes iter
+        let ch := ByteArray.peekc bytes iter
+        if ch = ASCII_D then
+          let iter := ByteArray.skip bytes iter
+          match parseDeletionLine bytes iter with
+          | .error _ => .error false
+          | .ok ⟨clauseIds, iter⟩ =>
+            match SR.consumeDeletionLine F clauseIds with
             | .error _ => .error false
-            | .ok ⟨clauseIds, iter⟩ =>
-              match SR.consumeDeletionLine F clauseIds with
-              | .error _ => .error false
-              | .ok F => loop iter ⟨F, τ, σ⟩
-          else
-            let F := Formula.commitClauseUntil F (lineId - 1)
-            match parseLSRAdditionLine F bytes iter with
-            | .error _ => .error false
-            | .ok ⟨iter, F, line⟩ =>
-              match SR.checkLine ⟨F, τ, σ⟩ line with
-              | .error b => .error b
-              | .ok ⟨F, τ, σ⟩ => loop iter ⟨F, τ, σ⟩
+            | .ok F => loop iter ⟨F, τ, σ⟩
         else
-          .ok (⟨F, τ, σ⟩, iter)
+          let F := Formula.commitClauseUntil F (lineId - 1)
+          match parseLSRAdditionLine F bytes iter with
+          | .error _ => .error false
+          | .ok ⟨iter, F, line⟩ =>
+            match SR.checkLine ⟨F, τ, σ⟩ line with
+            | .error b => .error b
+            | .ok ⟨F, τ, σ⟩ => loop iter ⟨F, τ, σ⟩
+      else
+        .ok (⟨F, τ, σ⟩, iter)
 
-      match loop iter ⟨F, τ, σ⟩ with
-      | .ok _ =>
-        IO.println "c Proof is valid, but did not derive the empty clause."
-        IO.println "s VALID"
-      | .error true => do
-        IO.println "c Proof derived the empty clause"
-        IO.println "s VERIFIED UNSAT"
-      | .error false => do
-        IO.println "c Error or invalid proof"
-        IO.println "s INVALID"
+    match loop iter ⟨F, τ, σ⟩ with
+    | .ok _ =>
+      IO.println "c Proof is valid, but did not derive the empty clause."
+      IO.println "s VALID"
+    | .error true => do
+      IO.println "c Proof derived the empty clause"
+      IO.println "s VERIFIED UNSAT"
+    | .error false => do
+      IO.println "c Error or invalid proof"
+      IO.println "s INVALID"
 
   | _ => printUsage
